sha/verif_hmac_final.v
@@ -1,0 +1,225 @@
+Require Import floyd.proofauto.
+Import ListNotations.
+Require sha.sha.
+Require sha.SHA256.
+Local Open Scope logic.
+
+Require Import sha.spec_sha.
+Require Import sha_lemmas.
+Require Import sha.HMAC_functional_prog.
+
+Require Import sha.hmac091c.
+Require Import sha.spec_hmac.
+
+Lemma withspacer_refl: forall sh a P, withspacer sh a a P = P.
+Proof. intros. unfold withspacer. 
+  rewrite <- Zminus_diag_reverse. trivial.
+Qed.
+
+Lemma body_hmac_sha256: semax_body Vprog Gtot
+       f_HMAC_Final HMAC_FinalWK_spec.
+Proof.
+start_function.
+name ctx' _ctx.
+name md' _md.
+simpl_stackframe_of. normalize.
+eapply semax_pre with (P':=PROP  ()
+   LOCAL  (`(eq md) (eval_id _md); `(eq c) (eval_id _ctx);
+   `(eq KV) (eval_var sha._K256 (tarray tuint 64)))
+   SEP 
+   ((EX b:_, local (`(eq b) (eval_var _buf (tarray tuchar 32)))
+             && `(data_at_ Tsh (tarray tuchar 32) b));
+   `(hmacstate_ h1 c); `(K_vector KV); `(memory_block shmd (Int.repr 32) md))).
+  entailer. apply exp_right with (x:=eval_var _buf (tarray tuchar 32) rho).
+  entailer.
+normalize. intros b. normalize.
+rewrite memory_block_isptr. unfold hmacstate_. normalize.
+rename H into WrshMD. 
+rename H0 into isPtrMD. 
+intros ST. normalize.
+destruct h1; simpl in *.
+destruct H as [reprMD [reprI [reprO [iShaLen [oShaLen [KeyST [l [KeylenST [KL ZLen]]]]]]]]].
+rewrite KL in *.
+erewrite (field_except_at_lemma _ _ _md_ctx nil); try reflexivity.
+simpl. 
+
+(*By rewriting with field_at_data_at here instead of inside the forward_call,
+  we remember facts SCc and ACc which are necessary for performing the
+  "inverse" conversion at the end of this proof*)  
+rewrite field_at_data_at; try reflexivity. simpl. normalize. simpl. 
+rename H into SCc. rename H0 into ACc.
+
+rewrite <- memory_block_data_at_ ; try reflexivity. normalize.
+rename H into ACb.
+remember (ctx, b, c, Tsh, Tsh, KV) as WITNESS.
+forward_call WITNESS.
+  { assert (FR: Frame = [
+      `(field_except_at Tsh t_struct_hmac_ctx_st _md_ctx [] (snd ST) c);
+      `(memory_block shmd (Int.repr 32) md)]).
+       subst Frame. reflexivity.
+    rewrite FR. clear FR Frame. 
+    subst WITNESS. entailer. 
+    cancel.
+    unfold sha256state_. apply exp_right with (x:= mdCtx ST). entailer.
+  }
+after_call. subst WITNESS. normalize. simpl. 
+
+eapply semax_pre with (P':=(PROP  ()
+   LOCAL  (`(eq b) (eval_var _buf (tarray tuchar 32));
+   `(eq md) (eval_id _md); `(eq c) (eval_id _ctx);
+   `(eq KV) (eval_var sha._K256 (tarray tuint 64)))
+   SEP  (`(K_vector KV); 
+   `(data_at Tsh t_struct_hmac_ctx_st (default_val sha.t_struct_SHA256state_st, snd ST) c);
+   `(data_block Tsh (sha_finish ctx) b);
+   `(memory_block shmd (Int.repr 32) md)))).
+  entailer. cancel. 
+  erewrite (field_except_at_lemma _ _ _md_ctx nil); try reflexivity. simpl.
+  rewrite field_at_data_at; try reflexivity. simpl. normalize.
+
+unfold_data_at 1%nat. (*qinxiang told me about this tactic - we need a list of all tactics!!!*)
+rewrite (field_at_data_at _ _ [_o_ctx]); try reflexivity.
+rewrite (field_at_data_at _ _ [_md_ctx]); try reflexivity.
+normalize. simpl.
+rewrite at_offset_data_at. 
+
+eapply semax_pre with (P':=
+  (PROP  ()
+   LOCAL  (`(eq b) (eval_var _buf (tarray tuchar 32));
+   `(eq md) (eval_id _md); `(eq c) (eval_id _ctx);
+   `(eq KV) (eval_var sha._K256 (tarray tuint 64)))
+   SEP 
+   (`(field_at Tsh t_struct_hmac_ctx_st [_key_length]
+        (fst (snd (snd (snd ST)))) c);
+   `(field_at Tsh t_struct_hmac_ctx_st [_key] (snd (snd (snd (snd ST)))) c);
+   `(data_at Tsh (nested_field_type2 t_struct_hmac_ctx_st [_o_ctx])
+       (fst (snd (snd ST)))
+       (offset_val
+          (Int.repr (nested_field_offset2 t_struct_hmac_ctx_st [_o_ctx])) c));
+   `(field_at Tsh t_struct_hmac_ctx_st [_i_ctx] (fst (snd ST)) c);
+   `(memory_block Tsh (Int.repr (sizeof (nested_field_type2 t_struct_hmac_ctx_st [_md_ctx]))) c);
+   `(K_vector KV);
+   `(data_block Tsh (sha_finish ctx) b);
+   `(memory_block shmd (Int.repr 32) md)))).
+  entailer. cancel.
+  eapply derives_trans. apply data_at_data_at_. reflexivity.
+  rewrite <- (memory_block_data_at_ Tsh (nested_field_type2 t_struct_hmac_ctx_st [_md_ctx]) (eq_refl _) (eq_refl _)).
+  entailer.
+
+destruct ST as [MD [iCTX [oCTX [KEYLENST KEYST]]]]. simpl in *.
+remember (Tsh, Tsh, c, offset_val
+          (Int.repr (nested_field_offset2 t_struct_hmac_ctx_st [_o_ctx])) c, 
+          (mkTrep t_struct_SHA256state_st oCTX)) as WITNESS.
+forward_call WITNESS.
+  { assert (FR: Frame = [
+      `(field_at Tsh t_struct_hmac_ctx_st [_key_length] KEYLENST c);
+      `(field_at Tsh t_struct_hmac_ctx_st [_key] KEYST c);
+      `(field_at Tsh t_struct_hmac_ctx_st [_i_ctx] iCTX c);
+      `(K_vector KV); `(data_block Tsh (sha_finish ctx) b);
+      `(memory_block shmd (Int.repr 32) md)]).
+       subst Frame. reflexivity.
+    rewrite FR. clear FR Frame. 
+    subst WITNESS. entailer. cancel.
+  }
+after_call. subst WITNESS. normalize. subst retval0. simpl. 
+
+assert (SFL: Zlength (sha_finish ctx) = 32). 
+  unfold sha_finish. destruct ctx. 
+  rewrite <- functional_prog.SHA_256'_eq, Zlength_correct, length_SHA256', Z2Nat.id. trivial.
+  unfold SHA256_DIGEST_LENGTH; omega.
+
+(*Call sha256Update*)
+(*apply seq_assoc.*)
+(*eapply semax_seq'.
+frame_SEP 0 5 6.
+*)
+remember (oSha, sha_finish ctx, c, b, Tsh, SHA256_DIGEST_LENGTH, KV) as WITNESS.
+forward_call WITNESS.
+  { assert (FR: Frame = [
+       `(data_at Tsh t_struct_SHA256state_st oCTX
+           (offset_val (Int.repr (nested_field_offset2 t_struct_hmac_ctx_st [_o_ctx])) c));
+       `(field_at Tsh t_struct_hmac_ctx_st [_key_length] KEYLENST c);
+       `(field_at Tsh t_struct_hmac_ctx_st [_key] KEYST c);
+       `(field_at Tsh t_struct_hmac_ctx_st [_i_ctx] iCTX c);
+        (*`(data_block Tsh (sha_finish ctx) b);*)
+       `(memory_block shmd (Int.repr 32) md)]).
+       subst Frame. reflexivity.
+    rewrite FR. clear FR Frame. 
+    subst WITNESS. entailer. 
+    apply andp_right. rewrite SFL. unfold SHA256_DIGEST_LENGTH. entailer.
+     rewrite oShaLen. simpl. entailer.
+    cancel.
+    unfold sha256state_. apply exp_right with (x:=oCTX).
+    entailer.
+  }
+after_call. subst WITNESS. normalize. remember (sha_finish ctx) as SF. 
+apply semax_pre with (P':=EX  x : s256abs,
+  (PROP  ()
+   LOCAL  (`(eq b) (eval_var _buf (tarray tuchar 32));
+   `(eq md) (eval_id _md); `(eq c) (eval_id _ctx);
+   `(eq KV) (eval_var sha._K256 (tarray tuint 64)))
+   SEP 
+   (`(fun a : environ =>
+      (PROP  (update_abs (firstn (Z.to_nat SHA256_DIGEST_LENGTH) SF) oSha x)
+       LOCAL ()
+       SEP  (`(K_vector KV); `(sha256state_ x c); `(data_block Tsh SF b))) a)
+      globals_only;
+   `(data_at Tsh t_struct_SHA256state_st oCTX
+       (offset_val
+          (Int.repr (nested_field_offset2 t_struct_hmac_ctx_st [_o_ctx])) c));
+   `(field_at Tsh t_struct_hmac_ctx_st [_key_length] KEYLENST c);
+   `(field_at Tsh t_struct_hmac_ctx_st [_key] KEYST c);
+   `(field_at Tsh t_struct_hmac_ctx_st [_i_ctx] iCTX c);
+   `(memory_block shmd (Int.repr 32) md)))).
+   entailer. rename x into a. apply exp_right with (x:=a).
+     entailer.
+  normalize.
+  apply extract_exists_pre. intros updSha. normalize.
+  rewrite firstn_precise. 
+  Focus 2. unfold  SHA256_DIGEST_LENGTH. simpl. subst SF. 
+        unfold sha_finish. destruct ctx.
+        rewrite <- functional_prog.SHA_256'_eq,length_SHA256'. trivial.
+  simpl.
+  unfold sha256state_. normalize. intros updShaST. normalize.
+  
+remember (updSha, md, c, shmd, Tsh, KV) as WITNESS.
+forward_call WITNESS.
+  { assert (FR: Frame = [ `(data_block Tsh SF b);
+      `(data_at Tsh t_struct_SHA256state_st oCTX
+         (offset_val (Int.repr (nested_field_offset2 t_struct_hmac_ctx_st [_o_ctx])) c));
+      `(field_at Tsh t_struct_hmac_ctx_st [_key_length] KEYLENST c);
+      `(field_at Tsh t_struct_hmac_ctx_st [_key] KEYST c);
+      `(field_at Tsh t_struct_hmac_ctx_st [_i_ctx] iCTX c)]).
+       subst Frame. reflexivity.
+    rewrite FR. clear FR Frame. 
+    subst WITNESS. entailer. 
+    cancel.
+    unfold sha256state_. 
+    apply exp_right with (x:=updShaST). entailer.
+  }
+after_call. subst WITNESS. normalize. simpl.
+
+forward.
+unfold data_at_.
+apply exp_right with (x:=sha_finish updSha).
+simpl_stackframe_of. simpl. normalize.
+apply exp_right with (x:=HMACabs updSha iSha oSha (Int.unsigned l) key).
+unfold data_block.
+normalize.
+apply andp_right. apply prop_right. split; trivial.
+  exists updSha; eauto.
+cancel. 
+rewrite SFL in *.
+erewrite (data_at__array_at_ Tsh tuchar 32 noattr). cancel.
+  2: omega. 2: reflexivity. 
+unfold hmacstateWK_, hmac_relateWK. normalize.
+apply exp_right with (x:=(updShaST, 
+                         (iCTX, (oCTX, (Vint l,map Vint (map Int.repr (HMAC_FUN.mkKey key))))))).
+simpl. normalize.
+apply andp_right.
+  apply prop_right. exists l; auto.
+unfold_data_at 3%nat.
+cancel.
+rewrite (field_at_data_at _ _ [_o_ctx]); try reflexivity.
+rewrite (field_at_data_at _ _ [_md_ctx]); try reflexivity.
+entailer.
+Qed.
